WIP

src/example/TemporalLogicFull.v
@@ -1,10 +1,70 @@
 From stdpp Require Import coPset gmap namespaces.
 From sflib Require Import sflib.
 From Fairness Require Import PCM IProp IPM IndexedInvariants.
-From Fairness Require Import ISim SimDefaultRA LiveObligations SimWeakest.
-From Fairness Require Import LogicSyntaxHOAS TemporalLogic.
-From iris Require Import bi.big_op.
-From iris Require base_logic.lib.invariants.
+From Fairness Require Import ISim SimDefaultRA LiveObligations SimWeakest LogicSyntaxHOAS.
+From Fairness Require Export TemporalLogic.
+From Fairness Require Import SCMem.
+(* From iris Require Import bi.big_op. *)
+(* From iris Require base_logic.lib.invariants. *)
 Require Import Program.
 
+Section XADEF.
 
+  Variant xatom :=
+    | scm_points_to (p v : SCMem.val)
+    | scm_points_tos (p : SCMem.val) (vs : list SCMem.val)
+    | scm_memory_black (m : SCMem.t)
+  .
+
+  Global Instance XAtom : AuxAtom := { aAtom := xatom }.
+
+End XADEF.
+
+Section XAINTERP.
+
+  Context `{Σ : GRA.t}.
+  (* SCMem related RAs *)
+  Context `{MEMRA: @GRA.inG memRA Σ}.
+
+  Definition xatom_sem (xa : xatom) : iProp :=
+    match xa with
+    | scm_points_to p v => points_to p v
+    | scm_points_tos p vs => points_tos p vs
+    | scm_memory_black m => memory_black m
+    end.
+
+  Global Instance XAInterp : AAInterp := { aaintp := xatom_sem }.
+
+End XAINTERP.
+
+(** Notations. *)
+Notation "'ax' s" := (⟨Atom.aux (AA:=XAtom) s⟩)%F (at level 90) : formula_scope.
+Notation "l ↦ v" := (ax (scm_points_to l v))%F (at level 90) : formula_scope.
+
+Section TL.
+
+  Context {STT : StateTypes}.
+
+  Context `{Σ : GRA.t}.
+  (* Context `{AAI : @AAInterp Σ AA}. *)
+  (* Invariant related default RAs *)
+  Context `{OWNESRA : @GRA.inG OwnEsRA Σ}.
+  Context `{OWNDSRA : @GRA.inG OwnDsRA Σ}.
+  Context `{IINVSETRA : @GRA.inG (IInvSetRA Formula) Σ}.
+  (* State related default RAs *)
+  Context `{THDRA: @GRA.inG ThreadRA Σ}.
+  Context `{STATESRC: @GRA.inG (stateSrcRA st_src_type) Σ}.
+  Context `{STATETGT: @GRA.inG (stateTgtRA st_tgt_type) Σ}.
+  Context `{IDENTSRC: @GRA.inG (identSrcRA id_src_type) Σ}.
+  Context `{IDENTTGT: @GRA.inG (identTgtRA id_tgt_type) Σ}.
+  (* Liveness logic related default RAs *)
+  Context `{OBLGRA: @GRA.inG ObligationRA.t Σ}.
+  Context `{EDGERA: @GRA.inG EdgeRA Σ}.
+  Context `{ONESHOTRA: @GRA.inG ArrowShotRA Σ}.
+  Context `{ARROWRA: @GRA.inG (@ArrowRA id_tgt_type Formula) Σ}.
+  (* SCMem related RAs *)
+  Context `{MEMRA: @GRA.inG memRA Σ}.
+
+  Global Instance TLSet : @IInvSet Σ (@Formula XAtom STT) := SynIISet.
+
+End TL.
